Final tidy ups and added licence - no changes to functionality

case-study/chart_1_buggy/source/util/Value.java
@@ -1,6 +1,0 @@
-package util;
-
-public abstract class Value {
-  abstract public boolean isNum();
-  abstract public boolean isStr();
-}
