inference-tool/scatter.py
@@ -1,0 +1,70 @@
+#!/usr/bin/env python3
+# -*- coding: utf-8 -*-
+"""
+Created on Mon Mar  1 14:17:46 2021
+
+@author: michael
+"""
+
+import pickle
+import matplotlib.pyplot as plt
+
+import random
+import numpy
+import pandas as pd
+
+homedir = "/home/michael/Documents/efsm-inference/inference-tool/results"
+systems = ["spaceInvaders"]
+metrics = ["t1", "prop"]
+
+with open(f'{homedir}/data.dic', 'rb') as f:
+    data = pd.read_pickle(f)
+
+# for metric in metrics:
+#     for system in systems:
+#         print(system, metric)
+        
+#         mint = ([col for col in data[system]['MINT'][metric]])
+#         gp = ([col for col in data[system]['gp'][metric]])
+        
+#         print("ok")
+        
+#         mint = [item for sublist in mint for item in sublist]
+#         gp = [item for sublist in gp for item in sublist]
+        
+#         count = {}
+#         for i in mint:
+#             if i not in count:
+#                 count[i] = 0
+#             count[i] += 1
+#         print(len(count))
+
+#         # print("gp > mint", sum([x > y for x, y in zip(gp, mint)]))
+#         # print("gp >= mint", sum([x >= y for x, y in zip(gp, mint)]))
+        
+#         # print([x for x in data['spaceInvaders'] if x['MINT']['sensitivity'] > x['gp']['sensitivity']])
+        
+#         bins = numpy.linspace(0, 1, 100)
+        
+#         plt.hist(mint, bins, alpha=0.5, label='MINT')
+#         plt.hist(gp, bins, alpha=0.5, label='GP')
+        
+#         plt.xlabel(metric)
+#         plt.ylabel("Frequency")
+#         plt.title(f"GP vs MINT {metric}")
+        
+
+        
+#         plt.legend(loc='upper left')
+#         plt.show()
+
+column = "states"
+instances = [(x, y, z) for x,y,z in zip(data['spaceInvaders']['MINT'][column], data['spaceInvaders']['gp'][column], data['spaceInvaders']['MINT'].index) if x > y]
+
+# instances = [(len([((i),j) for i, j in zip(x, y) if i > j]), z) for x, y, z in instances]
+
+ninstances = [(x, y, z) for x,y,z in zip(data['spaceInvaders']['MINT'][column], data['spaceInvaders']['gp'][column], data['spaceInvaders']['MINT'].index) if x < y]
+# print("\n".join([str(x) for x in ninstances]))
+print(len(ninstances))
+
+# print("\n".join([str(x) for x in instances]))
