inference-tool/ultrametric-gp-paper.py
@@ -1,0 +1,235 @@
+#!/usr/bin/env python3
+# -*- coding: utf-8 -*-
+"""
+Created on Tue Feb 11 15:05:24 2020
+
+@author: michael
+"""
+
+import json
+from numpy import mean
+import numpy as np
+import re
+import math
+import os
+from itertools import takewhile, dropwhile
+import pandas as pd
+import matplotlib.pyplot as plt
+from matplotlib import gridspec
+import pickle
+from scipy.stats import mannwhitneyu
+from matplotlib import rc, rcParams
+rc('text', usetex=True)
+
+rcParams.update(
+    {   
+    "text.usetex": True,                
+    "font.family": "sans-serif",
+    "text.latex.preamble" : r"\usepackage{cmbright}\usepackage[notmath]{sansmathfonts}"
+    }
+)
+
+runtime_re = re.compile("Completed in (\d+)h (\d+)m (\d+).\d+s")
+
+homedir = "/home/michael/Documents/efsm-inference/inference-tool/results"
+# homedir = "/home/michael/Documents/results"
+
+data = {
+    "liftDoors": {},
+    "spaceInvaders": {},
+    "drinks": {},
+    "spaceInvadersGuards": {}
+    }
+
+systems = ["drinks", "spaceInvadersGuards"]
+systems = ["liftDoors", "spaceInvaders"]
+
+
+def configs(p):
+    if p == "liftDoors":
+        return [
+            # 'pta',
+            # 'none',
+            'MINT',
+            'gp',
+            # 'obfuscated-time-none',
+            'obfuscated-time-gp'
+            ]
+    if p == "spaceInvaders":
+        return [
+            # 'pta',
+            # 'none',
+            'MINT',
+            'gp',
+            # 'obfuscated-aliens-none',
+            'obfuscated-aliens-gp',
+            # 'obfuscated-shields-none',
+            'obfuscated-shields-gp',
+            # 'obfuscated-x-none',
+            'obfuscated-x-gp',
+            # Extras
+            'obfuscated-aliens-x-gp',
+            'obfuscated-x-shields-gp',
+            'obfuscated-aliens-shields-gp'
+            ]
+    if p == "drinks" or p == "spaceInvadersGuards":
+        return [
+            'pta',
+            'none',
+            'gp',
+            'gp-distinguish'
+            ]
+    return sorted(list(data[p].keys()))
+
+
+def axesColour(ax):
+    ax.spines['bottom'].set_color('#dddddd')
+    ax.spines['top'].set_color('#dddddd') 
+    ax.spines['right'].set_color('#dddddd')
+    ax.spines['left'].set_color('#dddddd')
+    ax.tick_params(axis='x', color='#dddddd')
+    ax.tick_params(axis='y', color='#dddddd')
+
+
+def box1(column, program, cfgs, fname, title, ax1):
+    print(program, data[program].keys())
+    cfgs = [c for c in cfgs if c in data[program]]
+    if column == 'runtime':
+        cfgs = [c for c in cfgs if c != 'pta']
+    
+    if column == 't1' or column == "prop":
+        boxes_aux = [data[program][config][column] for config in cfgs]
+        boxes = [[item for sublist in l for item in sublist] for l in boxes_aux]
+    else:
+        boxes = [data[program][config][column].astype(float) for config in cfgs]
+    
+    ax1.boxplot(
+            boxes,
+            widths=0.4
+          )
+
+    labels = [" ".join(c.replace("obfuscated", "obfuscated\n").replace("pta", "PTA").replace("none", "without\npreprocessing").replace("distinguish", "\nguards").replace("gp", "GP").split("-")) for c in cfgs]
+    # ax1.set_xticks(range(0, len(labels)+1))
+    ax1.set_xticklabels(
+        labels,
+        rotation=30,
+        ha='right',
+        va='top',
+        ma='right',
+        rotation_mode="anchor"
+    )
+    ax1.tick_params(axis='both', labelsize=10)
+
+    axesColour(ax1)
+    ax1.set_title(title)
+    ax1.margins()
+    return boxes
+    
+def boxPlots(column, ps, fname, systems):
+    size = 0
+    for p in systems:
+        for c in ps[p]:
+            size += 1
+    
+    # fig1 = plt.figure(figsize=(0.8*size, 3))
+    # spec = gridspec.GridSpec(nrows=1, ncols=len(systems), width_ratios=[len(ps[p]) for p in systems])
+
+    fig, axs = plt.subplots(
+        nrows=1,
+        ncols=len(systems),
+        sharex='col',
+        sharey='row',
+        figsize=(0.8*size, 2.5),
+        gridspec_kw={'width_ratios': [len(ps[p]) for p in systems]}
+        )
+    # plt.subplots_adjust(wspace=0.08)
+    
+    print(f"box {fname}-{column} size: {size}")
+    
+    title = (
+        "Accepted Prefix" if column == "t1" else 
+        "NRMSE" if column == "nrmse" else 
+        "Runtime (Minutes)" if column == "runtime" else
+        column.capitalize()
+        )
+    
+    boxes = []
+    for i, p in enumerate(systems):
+        ax = axs[i]
+        ax.yaxis.set_tick_params(which='both', labelleft=True)
+
+        cfgs = configs(p)
+        
+        b = box1(column, p, cfgs, fname, r"\textsc{"+p+"} "+title, ax)
+        boxes.append(b)
+
+
+    # plt.tight_layout()
+    plt.savefig(f"{homedir}/graphs/{fname}.pdf", bbox_inches='tight')
+    plt.close()
+    return boxes
+
+
+if not os.path.exists(f"{homedir}/graphs"):
+    os.mkdir(f"{homedir}/graphs")
+
+
+# Load in the data from pickle if we can so we don't have to keep recalculating stuff
+with open(f'{homedir}/data.dic', 'rb') as f:
+    data = pickle.load(f)
+
+fname = "".join([p[:2] for p in systems])
+
+ps = {p:configs(p) for p in data}
+
+ls, ss = boxPlots("sensitivity", ps, f"{fname}-sensitivity-plots", systems)
+lt, st = boxPlots("t1", ps, f"{fname}-t1-plots", systems)
+
+
+cfgs = ["pta", "none", "gp", "MINT"]
+
+
+
+fig, ((ax1, ax2), (ax3, ax4)) = plt.subplots(
+        nrows=2,
+        ncols=2,
+        figsize=(0.9*11, 6),
+        gridspec_kw={'width_ratios': [3, 8], "wspace":0.12, "hspace":0.2}
+        )
+
+ax1.boxplot(ls, widths=0.4)
+ax1.title.set_text(r"\textsc{"+"liftDoors} "+' Sensitivity')
+ax2.boxplot(ss, widths=0.4)
+ax2.title.set_text(r"\textsc{"+"spaceInvaders} "+' Sensitivity')
+
+ax3.boxplot(lt, widths=0.4)
+ax3.title.set_text(r"\textsc{"+"liftDoors} "+' Accepted Prefix')
+ax3.set_xticklabels(
+    [" ".join(c.replace("obfuscated", "obfuscated\n").replace("pta", "PTA").replace("none", "without\npreprocessing").replace("distinguish", "\nguards").replace("gp", "GP").split("-")) for c in configs("liftDoors")],
+    rotation=30,
+    ha='right',
+    va='top',
+    ma='right',
+    rotation_mode="anchor"
+)
+
+ax4.boxplot(st, widths=0.4)
+ax4.title.set_text(r"\textsc{"+"spaceInvaders} "+' Accepted Prefix')
+ax4.set_xticklabels(
+    [" ".join(c.replace("obfuscated", "obfuscated\n").replace("pta", "PTA").replace("none", "without\npreprocessing").replace("distinguish", "\nguards").replace("gp", "GP").split("-")) for c in configs("spaceInvaders")],
+    rotation=30,
+    ha='right',
+    va='top',
+    ma='right',
+    rotation_mode="anchor"
+)
+
+ax1.xaxis.set_tick_params(which='major', labelleft=False)
+ax2.xaxis.set_tick_params(which='major', labelleft=False)
+
+for ax in fig.get_axes():
+    ax.yaxis.set_tick_params(which='both', labelleft=True)
+    ax.margins()
+    axesColour(ax)
+
+plt.savefig("/home/michael/Documents/papers/gp-paper/figures/graphs/lisp-plots.pdf", bbox_inches='tight')
