case-study/chart_1_buggy/ajc.sh
@@ -1,1 +1,0 @@
-ajc -1.6 -inpath .:build/:build-tests/:lib/junit.jar:lib/servlet.jar:lib/iText-2.1.4.jar -outxml -outjar lib/aspects.jar source/util/*.java
